Cert.v
@@ -1,4 +1,4 @@
-From iVM Require Import DSet Mono Cert0 Cert1.
+From iVM Require Import DSet Mono Cert0 Cert1 Cert2.
 Import DSetNotations.
 
 Unset Suggest Proof Using.
