Cert1.v
@@ -450,7 +450,7 @@ Proof.
   typeclasses eauto.
 Qed.
 
-#[global] Instance semiNeutral_defined a : SemiNeutral sndMixer (defined a).
+#[global] Instance semiNeutral_defined m a : SemiNeutral m (defined a).
 Proof.
   rewrite defined_spec.
   unfold SemiNeutral.
@@ -571,6 +571,11 @@ Proof.
     lia.
 Qed.
 
+Instance confined_assume' P {DP: Decidable P} : Confined (@fstMixer State) (assume' P).
+Proof.
+  typeclasses eauto.
+Qed.
+
 Lemma pop_defined :
   pop =
     let* sp := get' SP in
@@ -581,373 +586,199 @@ Proof.
   setoid_rewrite pop_spec.
   setoid_rewrite load_spec.
   smon_ext' SP sp.
+  setoid_rewrite lens_put_get.
+  setoid_rewrite lens_put_put.
+
+  setoid_rewrite (confined_get SP); [ | typeclasses eauto .. ].
+  setoid_rewrite lens_put_get.
+  setoid_rewrite (confined_put SP _); [ | typeclasses eauto .. ].
+  setoid_rewrite lens_put_put.
+
+  repeat setoid_rewrite bind_assoc.
+  repeat setoid_rewrite (confined_get MEM); [ | typeclasses eauto .. ].
+
+  smon_ext' MEM mem.
+  setoid_rewrite lens_put_get.
+
+  setoid_rewrite postpone_assume'.
+  setoid_rewrite (confined_get MEM); [ | typeclasses eauto .. ].
+  setoid_rewrite (confined_get MEM); [ | typeclasses eauto .. ].
+  setoid_rewrite lens_put_get.
+
+  change Machine.available' with available.
+
+  destruct (decide (available sp)) as [Hsp|Hsp].
+  - repeat setoid_rewrite ret_bind.
+    destruct (mem sp Hsp) as [x|].
+    + now setoid_rewrite ret_bind.
+    + rewrite extr_spec. now smon_rewrite01.
+
+  - now smon_rewrite01.
+Qed.
+
+Proposition pop_get_SP {X} (f: Cell -> B64 -> M X) :
+  let* x := pop in
+  let* sp := get' SP in
+  f x sp =
+    let* sp := get' SP in
+    let* x := pop in
+    f x (offset 1 sp).
+Proof.
+  rewrite pop_spec.
+  smon_rewrite01.
+  setoid_rewrite confined_load.
+  setoid_rewrite lens_put_get.
+  setoid_rewrite lens_get_get.
+  reflexivity.
+Qed.
+
+Instance semiNeutral_load a : SemiNeutral MEM (load a).
+Proof.
+  unfold SemiNeutral.
+  rewrite load_spec.
+  change Machine.available' with available.
+  destruct (decide (available a)) as [Ha|Ha]; [ | now smon_rewrite01 ].
+  setoid_rewrite ret_bind.
+  rewrite get_spec.
+  rewrite putM_spec.
+  rewrite extr_spec.
   smon_rewrite.
+  smon_ext s.
+  setoid_rewrite put_get'.
+  destruct (proj MEM s a Ha) as [x|]; [ | now smon_rewrite01 ].
+  smon_rewrite.
+Qed.
 
-  destruct (decide _) as [Hsp|Hsp].
-  - smon_rewrite.
-    setoid_rewrite (confined_get MEM).
+Instance semiNeutral_pop : SemiNeutral MEM pop.
+Proof.
+  unfold SemiNeutral.
+  rewrite pop_spec.
+  rewrite get_spec.
+  rewrite put_spec.
+  setoid_rewrite semiNeutral_load.
+  setoid_rewrite putM_specL.
+  smon_rewrite.
+Qed.
 
-    (* ------------ TODO: Continue from here -----------------*)
-
-    smon_ext' MEM mem.
-    smon_rewrite.
-
-
-
-    setoid_rewrite <- (confined_put SP sp).
-    setoid_rewrite <- (confined_put SP sp).
-
+Proposition sDefined_member a u (Hau: a ∈ u) :
+  sDefined u = defined a;; sDefined u.
+Proof.
+  rewrite sDefined_spec.
+  smon_ext' MEM mem.
+  setoid_rewrite (semiNeutral_get_put MEM (defined a)).
+  repeat setoid_rewrite lens_put_get.
+  rewrite defined_spec.
+  destruct (decide (available a)) as [Ha|Ha].
+  - smon_rewrite01.
+    repeat setoid_rewrite lens_put_get.
+    destruct (decide (mem a Ha)) as [Hm|Hm].
+    + smon_rewrite.
+    + smon_rewrite01.
+      destruct (decide _) as [H|H].
+      * contradict Hm.
+        specialize (H a Hau).
+        destruct H as [Ha' Hm].
+        destruct (is_true_unique Ha Ha').
+        exact Hm.
+      * smon_rewrite.
+  - smon_rewrite01.
+    destruct (decide _) as [H|H].
+    + contradict Ha.
+      specialize (H a Hau).
+      destruct H as [Ha Hm].
+      exact Ha.
+    + now smon_rewrite01.
+Qed.
 
 Lemma popMany_defined n :
   popMany n =
     let* sp := get' SP in
     sDefined (nAfter n sp);;
     popMany n.
-Proof.
+Proof. (* TODO: Simplify *)
   induction n.
   - simp popMany.
     setoid_rewrite nAfter_empty.
     setoid_rewrite sDefined_empty.
     smon_rewrite.
-  - match goal with |- _ = ?r => set (rh :=r) end.
-    simp popMany.
-    setoid_rewrite IHn.
 
-    smon_rewrite.
+  - simp popMany.
+    setoid_rewrite IHn at 1.
+    setoid_rewrite pop_defined at 1.
+    repeat setoid_rewrite bind_assoc.
 
-
-
-
-Proposition popMany_pushMany n :
-  let* u := popMany n in
-  pushMany u =
-    let* sp := get' SP in
-    sDefined (nAfter n sp).
-Proof.
-  unfold def, member.
-  smon_ext' SP sp.
-  setoid_rewrite lens_put_get.
-  smon_ext' MEM mem.
-  induction n.
-
-  - simp popMany. setoid_rewrite ret_bind. cbn.
-    rewrite pushMany_empty.
-    do 2 (apply bind_extensional; intros []).
-    rewrite <- sDefined_empty. f_equal.
-    apply extensionality. intros a. cbn.
-    split; [ tauto | ]. unfold member.
-    intros H. apply asBool_decide in H. destruct H. lia.
-
-  - setoid_rewrite popMany_S.
-    setoid_rewrite to_list_action.
-    setoid_rewrite pushMany_action.
-    setoid_rewrite pushMany_one.
-    setoid_rewrite (collapse_bind_lift pop_push).
-
-    smon_rewrite01.
-    setoid_rewrite (popMany_getSP n).
-    setoid_rewrite lens_put_get.
-
-    transitivity (
-      put' MEM mem;;
-      let* u := (put' SP sp;; popMany n) in
-      defined (toB64 (n + sp));;
-      pushMany u);
-    [ now smon_rewrite01 | ].
-
-    setoid_rewrite <- (confined_popMany sp n _).
-    + rewrite (semiNeutral_put_put MEM (defined _)).
-      rewrite bind_assoc.
-      setoid_rewrite IHn.
-      clear IHn.
-
-      setoid_rewrite nAfter_nonempty.
-      setoid_rewrite union_symmetric.
-
-      setoid_rewrite sDefined_union.
-      setoid_rewrite sDefined_singleton.
-      unfold offset.
-      rewrite <- (semiNeutral_put_put MEM (defined _)).
-      setoid_rewrite (confined_put SP) at 1.
-      * reflexivity.
-      * unshelve eapply (confined_neutral _ (Hmx := confined_defined _)).
-
-    + clear x. (* Where did this come from? *)
-      unshelve eapply (confined_neutral _ (Hmx := confined_defined _)).
-      set (a := toB64 _).
-      set (u := nAfter _ _).
-
-      assert (Independent (MEM' u) (MEM'' a)) as Hi.
-      * setoid_rewrite point_mem''.
-        unfold MEM'.
-        apply composite_independent_r.
-        apply separate_independent.
-        intros x [Hu Ha].
-        subst a u.
-        unfold nAfter, singleton, def, member in Hu, Ha.
-        apply asBool_decide in Hu, Ha.
-        destruct Hu as [i [Hi Hi']].
-        subst x.
-
-
-
-
-Qed.
-
-
-
-
-    symmetry.
-    destruct (decide _) as [H|H]; [ reflexivity | ].
-    contradict H. intros a.
-    destruct (decide _) as [HH|HH]; [ | easy ].
-    exfalso. destruct HH. lia.
-  - setoid_rewrite popMany_S.
-    setoid_rewrite to_list_action.
-    setoid_rewrite pushMany_action.
-    setoid_rewrite pushMany_one.
-    setoid_rewrite (collapse_bind_lift pop_push).
-
-    smon_rewrite01.
-    setoid_rewrite (popMany_getSP n).
-    setoid_rewrite lens_put_get.
-
-    transitivity (
-      put' MEM mem;;
-      let* u := (put' SP sp;; popMany n) in
-      defined (toB64 (n + sp));;
-      pushMany u).
-    + now smon_rewrite01.
-    + setoid_rewrite <- (confined_popMany sp n _);
-      [ | eapply (confined_neutral _ (Hmx := confined_defined _)) ].
-      rewrite (semiNeutral_put_put MEM (defined _)).
-      rewrite bind_assoc.
-      setoid_rewrite IHn.
-      clear IHn.
-      fold sDefined.
-
-
-
-
-Proposition popMany_pushMany n :
-  let* u := popMany n in
-  pushMany u =
-    let* sp := get' SP in
-    sDefined (nAfter n sp).
-Proof.
-  unfold nAfter, sDefined, def, member.
-  smon_ext' SP sp.
-  setoid_rewrite lens_put_get.
-  setoid_rewrite <- (confined_put SP _) at 2.
-  2: solve [typeclasses eauto].
-  smon_ext' MEM mem.
-  setoid_rewrite lens_put_get.
-  induction n.
-  - simp popMany. setoid_rewrite ret_bind. cbn.
-    rewrite pushMany_empty.
-    do 2 (apply bind_extensional; intros []).
-    destruct (decide _) as [H|H]; [ reflexivity | ].
-    contradict H. intros a.
-    destruct (decide _) as [HH|HH]; [ | easy ].
-    exfalso. destruct HH. lia.
-  - setoid_rewrite popMany_S.
-    setoid_rewrite to_list_action.
-    setoid_rewrite pushMany_action.
-    setoid_rewrite pushMany_one.
-    setoid_rewrite (collapse_bind_lift pop_push).
-
-    smon_rewrite01.
-    setoid_rewrite (popMany_getSP n).
-    setoid_rewrite lens_put_get.
-
-    transitivity (
-      put' MEM mem;;
-      let* u := (put' SP sp;; popMany n) in
-      defined (toB64 (n + sp));;
-      pushMany u).
-    + now smon_rewrite01.
-    + setoid_rewrite <- (confined_popMany sp n _);
-      [ | eapply (confined_neutral _ (Hmx := confined_defined _)) ].
-      rewrite (semiNeutral_put_put MEM (defined _)).
-      rewrite bind_assoc.
-      setoid_rewrite IHn.
-      clear IHn.
-      fold sDefined.
-
-
-
-
-
-
-      rewrite defined_spec.
-      destruct (decide (available _)) as [Hn|Hn].
-      2: {
-        smon_rewrite01.
-        set (d := decide _).
-        destruct d as [H|H]; [ | now smon_rewrite01 ].
-        exfalso.
-        set (a := toB64 (n + sp)) in *.
-        contradict Hn.
-        specialize (H a).
-        rewrite asBool_decide in H.
-        apply H.
-        exists n.
-        split; [ lia | reflexivity ].
-      }
-      smon_rewrite. (* TODO: slow! *)
-      destruct (mem _) as [Hn'|] eqn:en.
-      2: {
-        smon_rewrite01.
-        set (a := toB64 (n + sp)) in *.
-        set (d := decide _).
-        destruct d as [H|H]; [ | now smon_rewrite01 ].
-        exfalso.
-
-
-      }.
-      admit.
-
-
-
-
-        --
-
-          (spec)
-
-          Set Printing Coercions.
-          as_bool
-          rewrite (asBool_decide _) in H.
-
-
-          destruct H.
-
-
-        contradict H.
-
-        admit.
-        -- now smon_rewrite01.
-
-
-      rewrite <- (semiNeutral_put_put MEM (defined _)).
-      setoid_rewrite <- confined_defined; [ | typeclasses eauto ].
-      apply bind_extensional. intros [].
-      apply bind_extensional. intros [].
-
-
-
-
-
-
-      * admit.
-      * typeclasses eauto.
-
-      smon_rewrite. (* TODO: Very slow *)
-      rewrite <- bind_assoc.
-      setoid_rewrite bind_assoc at 2.
-
-      setoid_rewrite <- (semiNeutral_put_put MEM (defined _)).
-
-
-      rewrite (semiNeutral_get_put (X:=unit) MEM (defined _)).
-      smon_rewrite. (* TODO: Very slow *)
-      rewrite (semiNeutral MEM (semiNeutral_defined _)).
-      repeat setoid_rewrite bind_assoc.
-
-
-
-    match goal with [ |- _ = ?h ] => set (hs := h) end.
-
-
-    transitivity (
-      put' MEM mem;;
-      defined (toB64 (n + sp));;
-      put' MEM mem;;
-      let* u := (put' SP sp;; popMany n) in
-      pushMany u).
-    + setoid_rewrite <- (confined_popMany sp n _).
-
-    rewrite (lens_semiNeutral (sub_semiNeutral (semiNeutral_defined _) MEM)).
-      smon_rewrite.
-    sndMixer
-    setoid_rewrite <- confined_defined.
-      setoid_rewrite (confined_popMany sp n _).
-      smon_rewrite.
-
-
-
-
-    + now smon_rewrite01.
-    + setoid_rewrite <- (confined_popMany sp n _);
-      [ | eapply (confined_neutral _ (Hmx := confined_defined _)) ].
-
-
-
-
-
-
-    transitivity (
-      put' MEM mem;;
-      let* u := (put' SP sp;; popMany n) in
-      defined (toB64 (n + sp));;
-      pushMany u).
-    + now smon_rewrite01.
-    + setoid_rewrite <- (confined_popMany sp n _);
-      [ | eapply (confined_neutral _ (Hmx := confined_defined _)) ].
-
-
-
-
-      setoid_rewrite confined_defined.
-
-      repeat setoid_rewrite bind_assoc.
-      setoid_rewrite IHn.
-      setoid_rewrite <- confined_defined.
-      setoid_rewrite <- confined_defined.
-      * admit.
-      * typeclasses eauto.
-      *
-
-
-
-  by_lia (S n = (n + 1)%nat) as H.
-    setoid_rewrite H.
-
-    popMany_action
     smon_ext' SP sp.
     setoid_rewrite lens_put_get.
-    setoid_rewrite <- (confined_put SP _).
+    setoid_rewrite pop_get_SP.
+    setoid_rewrite (confined_get SP).
+    setoid_rewrite lens_put_get.
 
-    destruct (decide (forall a: B64, _)).
+    rewrite defined_spec.
+    destruct (decide (available sp)) as [Hsp|Hsp].
+    + smon_rewrite01.
+      setoid_rewrite (confined_get MEM); [ | typeclasses eauto ].
+      smon_ext' MEM mem.
+      setoid_rewrite lens_put_get.
 
+      destruct (decide (mem sp Hsp)) as [Hm|Hm].
+      * setoid_rewrite ret_tt_bind.
+        rewrite sDefined_spec.
+        smon_rewrite01.
+        setoid_rewrite (confined_get MEM) at 2; [ | typeclasses eauto ].
+        setoid_rewrite lens_put_get.
+        setoid_rewrite (semiNeutral_get_put MEM pop) at 1.
 
+        setoid_rewrite (confined_get MEM); [ | typeclasses eauto ].
+        repeat setoid_rewrite lens_put_get.
+        setoid_rewrite <- (confined_put MEM mem); [ | typeclasses eauto .. ].
+        setoid_rewrite <- semiNeutral_put_put; [ | typeclasses eauto .. ].
+        destruct (decide _) as [H1|H1];
+        destruct (decide _) as [H2|H2].
+        1,4: smon_rewrite.
+        -- contradict H2.
+          intros a Ha.
+          rewrite nAfter_spec in Ha.
+          destruct Ha as [i [Hi Hi']].
+          change (toB64 _) with (offset i sp) in Hi'.
+          by_lia (i = 0 \/ (i - 1) + 1 = i)%nat as Hii.
+          destruct Hii as [Hii|Hii].
+          ++ rewrite Hii in Hi'.
+            rewrite Z_action_zero in Hi'.
+            destruct Hi'. exists Hsp. exact Hm.
+          ++ apply H1. rewrite nAfter_spec.
+            exists (i - 1)%nat.
+            change (toB64 _) with (offset (i - 1)%nat (offset 1 sp)).
+            split.
+            ** lia.
+            ** rewrite <- Hi'.
+              rewrite <- Z_action_add.
+              f_equal.
+              lia.
+          -- contradict H1.
+            intros a Ha.
+            apply H2.
+            apply nAfter_tail.
+            exact Ha.
+      * smon_rewrite01.
+        setoid_rewrite (sDefined_member sp); [ | apply nAfter_head ].
+        setoid_rewrite bind_assoc.
+        setoid_rewrite <- (confined_put SP);
+          rewrite defined_spec;
+          [ | typeclasses eauto ].
+        decided Hsp.
+        smon_rewrite.
+        undecided Hm.
+        now smon_rewrite01.
 
+    + smon_rewrite01.
+      setoid_rewrite (sDefined_member sp); [ | apply nAfter_head ].
+      setoid_rewrite bind_assoc.
+      setoid_rewrite <- (confined_put SP);
+        rewrite defined_spec;
+        [ | typeclasses eauto ].
+      undecided Hsp.
+      now smon_rewrite01.
 
-    Transparent pushMany.
-    unfold pushMany.
-
-
-
-
-  setoid_rewrite popMany_spec.
-  smon_ext' SP sp.
-  smon_rewrite. (* TODO: Slow! *)
-  setoid_rewrite <- (confined_put SP _).
-  2, 3: apply (confined_neutral (m':=MEM)); typeclasses eauto.
-  smon_ext' MEM mem.
-  smon_rewrite.
-
-  setoid_rewrite loadMany_spec_fromMem.
-  smon_rewrite.
-
-
-
-  setoid_rewrite (assume'_proper _ _ (asBool_decide _)).
-  set (b := as_bool (decide _)).
-  setoid_rewrite (asBool_decide _).
-  induction n.
-  - simp popMany.
-  smon_rewrite.
-
-(* Continue from here *)
-
-Admitted.
+    + rewrite defined_spec.
+      typeclasses eauto.
+Qed.
