Cert2.v
@@ -1,0 +1,348 @@
+From iVM Require Import DSet Mono Cert0 Cert1.
+Import DSetNotations.
+
+Unset Suggest Proof Using.
+
+(* TODO: Place inside section or module. *)
+Import OpCodes.
+
+Local Notation not_terminated := (ret true) (only parsing).
+Local Notation terminated := (ret false) (only parsing).
+
+(*****************)
+
+(* TODO: Continue from here *)
+
+Proposition popMany_pushMany n :
+  let* u := popMany n in
+  pushMany u =
+    let* sp := get' SP in
+    sDefined (nAfter n sp).
+Proof.
+  unfold def, member.
+  smon_ext' SP sp.
+  setoid_rewrite lens_put_get.
+  smon_ext' MEM mem.
+  induction n.
+
+  - simp popMany. setoid_rewrite ret_bind. cbn.
+    rewrite pushMany_empty.
+    do 2 (apply bind_extensional; intros []).
+    rewrite <- sDefined_empty. f_equal.
+    apply extensionality. intros a. cbn.
+    split; [ tauto | ]. unfold member.
+    intros H. apply asBool_decide in H. destruct H. lia.
+
+  - setoid_rewrite popMany_S.
+    setoid_rewrite to_list_action.
+    setoid_rewrite pushMany_action.
+    setoid_rewrite pushMany_one.
+    setoid_rewrite (collapse_bind_lift pop_push).
+
+    smon_rewrite01.
+    setoid_rewrite (popMany_getSP n).
+    setoid_rewrite lens_put_get.
+
+    transitivity (
+      put' MEM mem;;
+      let* u := (put' SP sp;; popMany n) in
+      defined (toB64 (n + sp));;
+      pushMany u);
+    [ now smon_rewrite01 | ].
+
+    setoid_rewrite <- (confined_popMany sp n _).
+    + rewrite (semiNeutral_put_put MEM (defined _)).
+      rewrite bind_assoc.
+      setoid_rewrite IHn.
+      clear IHn.
+
+      setoid_rewrite nAfter_nonempty.
+      setoid_rewrite union_symmetric.
+
+      setoid_rewrite sDefined_union.
+      setoid_rewrite sDefined_singleton.
+      unfold offset.
+      rewrite <- (semiNeutral_put_put MEM (defined _)).
+      setoid_rewrite (confined_put SP) at 1.
+      * reflexivity.
+      * unshelve eapply (confined_neutral _ (Hmx := confined_defined _)).
+
+    + clear x. (* Where did this come from? *)
+      unshelve eapply (confined_neutral _ (Hmx := confined_defined _)).
+      set (a := toB64 _).
+      set (u := nAfter _ _).
+
+      assert (Independent (MEM' u) (MEM'' a)) as Hi.
+      * setoid_rewrite point_mem''.
+        unfold MEM'.
+        apply composite_independent_r.
+        apply separate_independent.
+        intros x [Hu Ha].
+        subst a u.
+        unfold nAfter, singleton, def, member in Hu, Ha.
+        apply asBool_decide in Hu, Ha.
+        destruct Hu as [i [Hi Hi']].
+        subst x.
+
+
+
+
+Qed.
+
+
+
+
+    symmetry.
+    destruct (decide _) as [H|H]; [ reflexivity | ].
+    contradict H. intros a.
+    destruct (decide _) as [HH|HH]; [ | easy ].
+    exfalso. destruct HH. lia.
+  - setoid_rewrite popMany_S.
+    setoid_rewrite to_list_action.
+    setoid_rewrite pushMany_action.
+    setoid_rewrite pushMany_one.
+    setoid_rewrite (collapse_bind_lift pop_push).
+
+    smon_rewrite01.
+    setoid_rewrite (popMany_getSP n).
+    setoid_rewrite lens_put_get.
+
+    transitivity (
+      put' MEM mem;;
+      let* u := (put' SP sp;; popMany n) in
+      defined (toB64 (n + sp));;
+      pushMany u).
+    + now smon_rewrite01.
+    + setoid_rewrite <- (confined_popMany sp n _);
+      [ | eapply (confined_neutral _ (Hmx := confined_defined _)) ].
+      rewrite (semiNeutral_put_put MEM (defined _)).
+      rewrite bind_assoc.
+      setoid_rewrite IHn.
+      clear IHn.
+      fold sDefined.
+
+
+
+
+Proposition popMany_pushMany n :
+  let* u := popMany n in
+  pushMany u =
+    let* sp := get' SP in
+    sDefined (nAfter n sp).
+Proof.
+  unfold nAfter, sDefined, def, member.
+  smon_ext' SP sp.
+  setoid_rewrite lens_put_get.
+  setoid_rewrite <- (confined_put SP _) at 2.
+  2: solve [typeclasses eauto].
+  smon_ext' MEM mem.
+  setoid_rewrite lens_put_get.
+  induction n.
+  - simp popMany. setoid_rewrite ret_bind. cbn.
+    rewrite pushMany_empty.
+    do 2 (apply bind_extensional; intros []).
+    destruct (decide _) as [H|H]; [ reflexivity | ].
+    contradict H. intros a.
+    destruct (decide _) as [HH|HH]; [ | easy ].
+    exfalso. destruct HH. lia.
+  - setoid_rewrite popMany_S.
+    setoid_rewrite to_list_action.
+    setoid_rewrite pushMany_action.
+    setoid_rewrite pushMany_one.
+    setoid_rewrite (collapse_bind_lift pop_push).
+
+    smon_rewrite01.
+    setoid_rewrite (popMany_getSP n).
+    setoid_rewrite lens_put_get.
+
+    transitivity (
+      put' MEM mem;;
+      let* u := (put' SP sp;; popMany n) in
+      defined (toB64 (n + sp));;
+      pushMany u).
+    + now smon_rewrite01.
+    + setoid_rewrite <- (confined_popMany sp n _);
+      [ | eapply (confined_neutral _ (Hmx := confined_defined _)) ].
+      rewrite (semiNeutral_put_put MEM (defined _)).
+      rewrite bind_assoc.
+      setoid_rewrite IHn.
+      clear IHn.
+      fold sDefined.
+
+
+
+
+
+
+      rewrite defined_spec.
+      destruct (decide (available _)) as [Hn|Hn].
+      2: {
+        smon_rewrite01.
+        set (d := decide _).
+        destruct d as [H|H]; [ | now smon_rewrite01 ].
+        exfalso.
+        set (a := toB64 (n + sp)) in *.
+        contradict Hn.
+        specialize (H a).
+        rewrite asBool_decide in H.
+        apply H.
+        exists n.
+        split; [ lia | reflexivity ].
+      }
+      smon_rewrite. (* TODO: slow! *)
+      destruct (mem _) as [Hn'|] eqn:en.
+      2: {
+        smon_rewrite01.
+        set (a := toB64 (n + sp)) in *.
+        set (d := decide _).
+        destruct d as [H|H]; [ | now smon_rewrite01 ].
+        exfalso.
+
+
+      }.
+      admit.
+
+
+
+
+        --
+
+          (spec)
+
+          Set Printing Coercions.
+          as_bool
+          rewrite (asBool_decide _) in H.
+
+
+          destruct H.
+
+
+        contradict H.
+
+        admit.
+        -- now smon_rewrite01.
+
+
+      rewrite <- (semiNeutral_put_put MEM (defined _)).
+      setoid_rewrite <- confined_defined; [ | typeclasses eauto ].
+      apply bind_extensional. intros [].
+      apply bind_extensional. intros [].
+
+
+
+
+
+
+      * admit.
+      * typeclasses eauto.
+
+      smon_rewrite. (* TODO: Very slow *)
+      rewrite <- bind_assoc.
+      setoid_rewrite bind_assoc at 2.
+
+      setoid_rewrite <- (semiNeutral_put_put MEM (defined _)).
+
+
+      rewrite (semiNeutral_get_put (X:=unit) MEM (defined _)).
+      smon_rewrite. (* TODO: Very slow *)
+      rewrite (semiNeutral MEM (semiNeutral_defined _)).
+      repeat setoid_rewrite bind_assoc.
+
+
+
+    match goal with [ |- _ = ?h ] => set (hs := h) end.
+
+
+    transitivity (
+      put' MEM mem;;
+      defined (toB64 (n + sp));;
+      put' MEM mem;;
+      let* u := (put' SP sp;; popMany n) in
+      pushMany u).
+    + setoid_rewrite <- (confined_popMany sp n _).
+
+    rewrite (lens_semiNeutral (sub_semiNeutral (semiNeutral_defined _) MEM)).
+      smon_rewrite.
+    sndMixer
+    setoid_rewrite <- confined_defined.
+      setoid_rewrite (confined_popMany sp n _).
+      smon_rewrite.
+
+
+
+
+    + now smon_rewrite01.
+    + setoid_rewrite <- (confined_popMany sp n _);
+      [ | eapply (confined_neutral _ (Hmx := confined_defined _)) ].
+
+
+
+
+
+
+    transitivity (
+      put' MEM mem;;
+      let* u := (put' SP sp;; popMany n) in
+      defined (toB64 (n + sp));;
+      pushMany u).
+    + now smon_rewrite01.
+    + setoid_rewrite <- (confined_popMany sp n _);
+      [ | eapply (confined_neutral _ (Hmx := confined_defined _)) ].
+
+
+
+
+      setoid_rewrite confined_defined.
+
+      repeat setoid_rewrite bind_assoc.
+      setoid_rewrite IHn.
+      setoid_rewrite <- confined_defined.
+      setoid_rewrite <- confined_defined.
+      * admit.
+      * typeclasses eauto.
+      *
+
+
+
+  by_lia (S n = (n + 1)%nat) as H.
+    setoid_rewrite H.
+
+    popMany_action
+    smon_ext' SP sp.
+    setoid_rewrite lens_put_get.
+    setoid_rewrite <- (confined_put SP _).
+
+    destruct (decide (forall a: B64, _)).
+
+
+
+
+    Transparent pushMany.
+    unfold pushMany.
+
+
+
+
+  setoid_rewrite popMany_spec.
+  smon_ext' SP sp.
+  smon_rewrite. (* TODO: Slow! *)
+  setoid_rewrite <- (confined_put SP _).
+  2, 3: apply (confined_neutral (m':=MEM)); typeclasses eauto.
+  smon_ext' MEM mem.
+  smon_rewrite.
+
+  setoid_rewrite loadMany_spec_fromMem.
+  smon_rewrite.
+
+
+
+  setoid_rewrite (assume'_proper _ _ (asBool_decide _)).
+  set (b := as_bool (decide _)).
+  setoid_rewrite (asBool_decide _).
+  induction n.
+  - simp popMany.
+  smon_rewrite.
+
+(* Continue from here *)
+
+Admitted.
